tests/monadic/stmonad/STMonadtest.v
@@ -1,4 +1,5 @@
 
+(* TODO: optimize imports *)
 From Crane Require Import Monads.STMonad.   
 
 From Stdlib Require Import
@@ -42,205 +43,32 @@ From ITree Require Import
   ITreeFacts
 .
 
-Import Monads.
-Import ListNotations.
-Import ProperNotations.
-Local Open Scope monad_scope.
-Local Open Scope string_scope.
-
-
-
-  
-
-Section NatExampleTrees.
-
-  Context {E : Type -> Type}.
-  Context {T : Type}.
-  Context {ltu : T -> T -> Prop}.
-  Context `{Ix_Correct T ltu}.
-  Context {HST: STRefClass T}.
-
-  Let V : T -> Type := fun _ => nat. (* Nats only for this example. *)
-  Let S := unit.
-  Let E0 := (STEvent T S V) +' exceptE Err.
-
-
-  Definition new_and_read_both_nat : itree E0 (nat * nat) :=
-      r1 <- newSTRef zero 5 ;;
-      r2 <- newSTRef (suc zero) 6 ;; (* TODO: autogenerate successive indices? *)
-      x1 <- readSTRef r1 ;;
-      x2 <- readSTRef r2 ;;
-      Ret (x1, x2).
-
-  Definition tree_simp_nat : itree E0 nat :=
-    v <- newSTRef zero 5;;
-    readSTRef v.
-
-  (* NOTE: this failing definition is intentional.
-    The intent is to test that we don't allow reference indices to escape. *)
-  Fail Definition tree_escape_nat : itree E0 nat :=
-    v <- newSTRef 5;;
-    writeSTRef v (match v with mkSTRef _ _ idx => idx end);;
-    readSTRef v.
-
-  Definition tree_simp_another_nat : itree E0 nat :=
-    v <- newSTRef zero 5;;
-    writeSTRef v 6;;
-    val <- readSTRef v;;
-    Ret val.
-
-
-   Definition swap' (v w : STRef S nat) : itree E0 unit :=
-    a <- @readSTRef E0 T S  _ V  _ (STRefToIx _ _ v) v;;
-    b <- @readSTRef E0 T S _ V _ (STRefToIx _ _ w) w;;
-    writeSTRef v b;;
-    writeSTRef w a.
-
-  (* "swap" function from "Lazy Functional State Threads", by John Launchbury and Simon L Peyton Jones. *)
-  (* TODO: would be good for indices here to be inferrable. *)
-  Fail Definition swap (v w : STRef S nat) : itree E0 unit :=
-    a <- readSTRef v;;
-    b <- readSTRef w;;
-    writeSTRef v b;;
-    writeSTRef w a.
-
-
-  Definition array_simp_fixed_init : itree E0 nat :=
-    arr <- newArray zero zero (suc (suc (suc (suc (suc zero))))) 5;;
-    elem <- @readArray E0 T _ _ _ _ _ arr (suc (zero));;
-    Ret elem. 
-  
-  Definition array_simp_list : itree E0 (nat * nat * list nat) :=
-    arr <- newListArray zero zero (suc (suc (suc zero))) [5;4;3;2];;
-    elem <- @readArray _ _ _ _ _ _ zero arr zero;;
-    lst <- @getElems _ _ _ _ _ _ zero arr;;
-    Ret (elem, length lst, lst). 
-
-
-  (* source: https://wiki.haskell.org/Monad/ST *)
-  (* TODO: should not have to manually place indices as arguments. *)
-  Definition fibST (n : nat) : itree E0 nat :=
-    let fix fibST' (n : nat) (x y : STRef S nat) (idx_x idx_y : T) : itree E0 nat :=
-      match n with
-      | 0 => @readSTRef _ _ _ _ _ _ idx_x x
-      | Datatypes.S n =>
-          x' <- @readSTRef _ _ _  _ _ _ idx_x x;;
-          y' <- @readSTRef _ _ _ _ _ _ idx_y y;;
-          @writeSTRef _ _ _ _ _ _ idx_x x y';;
-          @writeSTRef _ _ _ _ _ _ idx_y y (x' + y');;
-          fibST' n x y idx_x idx_y
-      end in
-    if (Nat.leb n 2)
-    then Ret n
-    else
-      x <- newSTRef zero 0;;
-      y <- newSTRef (suc zero) 1;;
-      fibST' n x y zero (suc zero).
-
-  Definition fibFun (n : nat) : nat :=
-    let fix fib' (n : nat) :=
-      match n with
-      | 0 => 0
-      | 1 => 1
-      | Datatypes.S (Datatypes.S m as m0) => fib' m0 + fib' m
-      end in
-    fib' n.
-
-  Section QSort. 
-
-  Definition swap_arr (arr : STArray T S nat) (left : T) (right : T) : itree E0 unit :=
-    leftVal <- readArray arr left;;
-    rightVal <- readArray arr right;;
-    @writeArray E0 T S _ _ _ zero arr left rightVal;;
-    @writeArray E0 T S _ _ _ (suc zero) arr right leftVal.
-
-  Definition forEachWith {A B} (xs : list A) (v : B) (f : B -> A -> itree E0 B)
-    : itree E0 B := foldM (flip f) (Ret v) xs.
-
-
-  Definition partition (arr : STArray T S nat) (arr_idx : T) (left : T) (right : T) (pivotIndex : T) : itree E0 T :=
-    pivotValue <- @readArray _ _ _ _ _ _ arr_idx arr pivotIndex;;
-    swap_arr arr pivotIndex right;;
-    storeIndex <- forEachWith (range left (sub right (suc zero))) left (fun i storeIndex =>
-        val <- @readArray _ _ _ _ _ _ arr_idx arr i;;
-        if (Nat.leb val pivotValue)
-            then swap_arr arr i storeIndex;;
-                 Ret (suc storeIndex)
-            else Ret storeIndex );;
-    swap_arr arr storeIndex right;;
-    Ret storeIndex.
-
-
-  (* TODO: define with equations. *)
-  (* Measure will be distance of the two pivots. *)
-  (* Try cofix! *)
-  Fail Fixpoint qsort (arr : STArray T S nat) (arr_idx : T) (left : T) (right : T) : itree E0 (STArray T S nat) :=
-    let leftn := toNat left in
-    let rightn := toNat right in 
-    let pivotIndexn := leftn + ((rightn - leftn) / 2) in
-    newPivot <- partition arr arr_idx left right (fromNat pivotIndexn);;
-    qsort arr arr_idx left (fromNat ((toNat newPivot) + 1));;
-    qsort arr arr_idx (fromNat ((toNat newPivot) + 1)) right.
-
-    
-  End QSort.
-
-  
-End NatExampleTrees.
-
-
+From CraneTestsMonadic.stmonad Require Import STMonadExamples.
 
 Module STMonadTests. 
   (* Re-exporting instances so they're available to call in the exported file. *)
   (* Just referring to them does not seem to work to extract them here, unfolding does *)
   Definition nat_idx : @Ix nat Nat.le := Eval unfold nat_ix in nat_ix.
   Definition nat_stref : STRefClass nat := Eval unfold nat_ix_stref in nat_ix_stref.
+
+  Definition array_simp_fixed_init := Eval unfold array_simp_fixed_init in (@array_simp_fixed_init nat unit Nat.le).
+  Definition array_simp_list := Eval unfold array_simp_list in (@array_simp_list nat unit Nat.le).
+  Definition fibST := Eval unfold fibST in (@fibST nat unit Nat.le).
+  Definition fibFun := Eval unfold fibFun in fibFun.
+  Definition list_hd := List.hd.
+  Definition list_tl := List.tl.
+  Definition new_and_read_both_bool := Eval unfold new_and_read_both_bool in (@new_and_read_both_bool nat unit Nat.le).
+  Definition new_and_read_both_nat := Eval unfold new_and_read_both_nat in (@new_and_read_both_nat nat unit Nat.le).
+  Definition tree_simp_another_nat := Eval unfold tree_simp_another_nat in (@tree_simp_another_nat nat unit Nat.le).
+  Definition tree_simp_bool := Eval unfold tree_simp_bool in (@tree_simp_bool nat unit Nat.le).
+  Definition tree_simp_nat := Eval unfold tree_simp_nat in (@tree_simp_nat nat unit Nat.le).
+  (* qsort TODO: extract qsort! *)
+
 End STMonadTests.
 
 
-Section BoolExampleTrees.
-
-  Context {E : Type -> Type}.
-  Context {T : Type}.
-  Context {ltu : T -> T -> Prop}.
-  Context `{Ix_Correct T ltu}.
-  Context {HST: STRefClass T}.
-
-  Let V : T -> Type := fun _ => bool. (* bools only for this example. *)
-  Let S := unit.
-  Let E0 := (STEvent T S V) +' exceptE Err.
-
-
-  Definition new_and_read_both_bool : itree E0 (bool * bool) :=
-      r1 <- newSTRef zero false ;;
-      r2 <- newSTRef (suc zero) true ;; 
-      x1 <- readSTRef r1 ;;
-      x2 <- readSTRef r2 ;;
-      Ret (x1, x2).
-
-  Definition tree_simp_bool : itree E0 bool :=
-    v <- newSTRef zero true;;
-    readSTRef v.
-
-End BoolExampleTrees.
-
-Definition list_hd {A} := @List.hd A.
-Definition list_tl {A} := @List.tl A.
-
 Require Import Crane.Mapping.NatIntStd.
 
-Set Crane Loopify.
 
-Crane Extraction "stmonad"
-  STMonadTests
-  new_and_read_both_nat
-  tree_simp_nat
-  tree_simp_another_nat
-  array_simp_fixed_init
-  list_hd
-  list_tl
-  array_simp_list
-  new_and_read_both_bool
-  tree_simp_bool
-  fibST
-  fibFun.
+
+Crane Extraction "stmonad" STMonadTests.
