tests/monadic/stmonad/STMonadDeriveTest.v
@@ -1,0 +1,323 @@
+(* Equational theory and Derive proofs for the ST monad *)
+
+From Crane Require Import Monads.STMonad Monads.ITree Monads.STMonadFacts.
+
+From Stdlib Require Import
+  Arith.PeanoNat
+  List
+  RelationClasses
+  Setoid
+  Strings.String
+  Classes.EquivDec
+.
+
+
+From ExtLib Require Import
+  CmpDec
+  Data.List
+  Data.Map.FMapAList
+  Data.Monads.EitherMonad
+  Data.Pair
+  Structures.Functor
+  Structures.Maps
+  Structures.Traversable
+  Structures.Reducible
+.
+
+From Paco Require Import paco.
+
+From ITree Require Import
+  Basics.HeterogeneousRelations
+  Eq.Paco2
+  Events.Exception
+  Events.FailFacts
+  Events.MapDefault
+  Events.MapDefaultFacts
+  Events.State
+  Events.StateFacts
+  ITree
+  ITreeFacts
+.
+
+Import Monads.
+Import ListNotations.
+Local Open Scope monad_scope.
+
+From Corelib Require Derive.
+From CraneTestsMonadic.stmonad Require Import STMonadExamples.
+
+Section EquationalTheory.
+  
+  Context {E : Type -> Type}.
+
+  Lemma eutt_fmap {R U : Type} {t1 t2 : itree E R} {f : R -> U} :
+    t1 ≈ t2 ->
+    fmap f t1 ≈ fmap f t2.
+    Proof using Type.
+      intros t_eq. apply eqit_map with (RR := eq).
+      + intros.
+        f_equal. assumption.
+      + apply t_eq.
+    Qed.
+
+  Lemma eutt_eq_bind {U R} (t : itree E U) (k1 k2: U -> itree E R):
+    (forall u, (k1 u) ≈ (k2 u)) ->
+    (ITree.bind t k1) ≈ (ITree.bind t k2).
+  Proof using Type. apply eutt_eq_bind. Qed.
+
+  Lemma eutt_eq_bind' {U R}
+    (k1 k2: U -> itree E R)
+    (t1 t2: itree E U):
+    t1 ≈ t2 ->
+    (forall u, (k1 u) ≈ (k2 u)) ->
+    (ITree.bind t1 k1) ≈ (ITree.bind t2 k2).
+  Proof. apply eutt_eq_bind'. Qed.
+
+
+Theorem bind_Ret_l : forall A B (f : A -> itree E B) (x : A), bind (Ret x) f ≈ f x.
+  setoid_rewrite Ret_is_ret.
+  setoid_rewrite Monad.bind_ret_l.
+  reflexivity.
+  Qed.
+          
+
+Theorem bind_Ret_r : forall A (x : itree E A), bind x (fun y => Ret y) ≈ x.
+  intros A x. setoid_rewrite Monad.bind_ret_r. reflexivity. Qed.
+
+End EquationalTheory.
+
+
+Ltac refine_prod :=
+  (refine (fun '(a,b) => _)).
+
+Ltac refine_arg :=
+  (refine (fun arg => _)).
+
+Ltac refine_arg2 :=
+  (refine (fun arg1 arg2 => _)).
+
+
+Ltac monad_simpl_inner :=
+  repeat (repeat setoid_rewrite Monad.bind_bind;
+          repeat setoid_rewrite bind_Ret_l;
+          repeat setoid_rewrite bind_Ret_r).
+
+
+
+(* Useful for lifting ITree's back to a monad instance. *)
+Ltac change_to_monad :=
+  change (@ITree.bind ?E) with (@Monad.bind (itree E) _);
+  try setoid_rewrite Ret_is_ret.
+
+Ltac bind_split_refl_intros split_tactic :=
+  split_tactic ;[ reflexivity | intros]
+  ;cbv beta match.
+
+Section DeriveProofs.
+
+
+  Let T := nat.
+  Let ltu := Nat.le.
+  Existing Instance nat_ix_correct.
+  Existing Instance nat_ix_stref.
+  Context {S : Type}.
+  
+  (* only integer typed values here *)
+  Let V : T -> Type := fun _ => nat.
+
+  Let E0 := (STEvent T S V) +' exceptE Err.
+
+
+  Transparent HAList.halist_lookup HAList.halist_add HAList.HMap_halist HAList.HMapOk_halist.
+
+  Derive (tree_simplified : itree (exceptE Err) nat) in
+    ( runST (S := S) (fun S => tree_simp_nat)
+        ≈
+      tree_simplified
+    ) as tree_simplification.
+  Proof.
+    unfold runST.
+    unfold tree_simp_nat.
+    etransitivity.
+    { eapply eutt_fmap.
+      eapply (eutt_eq_bind_interp_st ltu ltac:(refine_prod)).
+      - unfold newSTRef.
+        rewrite interp_st_trigger.
+        cbn.
+        reflexivity.
+      - intros u lmem'.
+        unfold readSTRef.
+        rewrite interp_st_trigger.
+        cbn.
+        reflexivity. }
+    setoid_rewrite map_bind.
+    repeat setoid_rewrite bind_Ret_l.
+    simpl.
+    unfold tree_simplified.
+    reflexivity.
+  Defined.
+
+
+
+  Derive (readboth_simplified : itree (exceptE Err) (nat*nat)) in
+    ( runST (S := S) (fun S => new_and_read_both_nat)
+        ≈
+      readboth_simplified
+    ) as tree_simplification2.
+  Proof.
+    unfold runST, new_and_read_both_nat.
+    etransitivity.
+    { eapply eutt_fmap.
+      eapply (eutt_eq_bind_interp_st ltu ltac:(refine_prod)).
+      - unfold newSTRef. rewrite interp_st_trigger. cbn. reflexivity.
+      - intros u lmem'.
+        eapply (eutt_eq_bind_interp_st ltu ltac:(refine_arg)).
+        + unfold newSTRef. rewrite interp_st_trigger. cbn.
+          change lmem' with (fst (lmem', u)). reflexivity.
+        + intros ? ?.
+          eapply (eutt_eq_bind_interp_st ltu ltac:(refine_arg)).
+          * unfold readSTRef. rewrite interp_st_trigger. cbn.
+            change u with (snd (lmem', u)).
+            change lmem'0 with (fst (lmem'0, u0)). reflexivity.
+          * intros ? ?.
+            eapply (eutt_eq_bind_interp_st ltu ltac:(refine_arg)).
+            -- unfold readSTRef. rewrite interp_st_trigger. cbn.
+               change u with (snd (lmem', u)).
+               change lmem'0 with (fst (lmem'0, u0)).
+               change u0 with (snd (lmem'0, u0)).
+               change lmem'1 with (fst (lmem'1, u1)). reflexivity.
+            -- intros ? ?.
+               rewrite interp_st_Ret.
+               change lmem'2 with (fst (lmem'2, u2)).
+               change u1 with (snd (lmem'1, u1)).
+               change u2 with (snd (lmem'2, u2)). reflexivity. }
+    setoid_rewrite map_bind.
+    repeat setoid_rewrite bind_Ret_l.
+    simpl.
+    unfold readboth_simplified.
+    reflexivity.
+  Defined.
+
+  
+  Derive (read_array5 : itree (exceptE Err) nat) in
+    ( runST (S := S) (fun S => array_simp_fixed_init)
+        ≈
+      read_array5
+    ) as tree_simplification3.
+  Proof.
+    unfold runST, array_simp_fixed_init.
+    etransitivity.
+    { eapply eutt_fmap.
+      eapply (eutt_eq_bind_interp_st ltu ltac:(refine_prod)).
+      {
+        unfold newArray. rewrite interp_st_trigger. cbn. reflexivity.
+      }
+      intros ? ?.
+      eapply (eutt_eq_bind_interp_st ltu ltac:(refine_arg)).
+      {
+        unfold readArray. rewrite interp_st_trigger. cbn. reflexivity.
+      }
+      intros ? ?.
+      rewrite interp_st_Ret. reflexivity.
+    }
+    setoid_rewrite map_bind.
+    repeat setoid_rewrite bind_Ret_l.
+    simpl.
+    unfold read_array5.
+    reflexivity.
+    Defined.
+
+  Derive (read_array_list_init : itree (exceptE Err) (nat * nat * list nat)) in
+    ( runST (S := S) (fun S => array_simp_list)
+        ≈
+      read_array_list_init
+    ) as tree_simplification4.
+  Proof.
+    unfold runST, array_simp_fixed_init.
+    etransitivity.
+    { eapply eutt_fmap.
+      eapply (eutt_eq_bind_interp_st ltu ltac:(refine_prod)).
+      {
+        unfold newListArray. rewrite interp_st_trigger. cbn. reflexivity.
+      }
+      intros ? ?.
+      eapply (eutt_eq_bind_interp_st ltu ltac:(refine_prod)).
+      {
+        unfold readArray. rewrite interp_st_trigger. cbn. reflexivity.
+      }
+      intros ? ?.
+      eapply (eutt_eq_bind_interp_st ltu ltac:(refine_prod)).
+      {
+        unfold getElems. rewrite interp_st_trigger. cbn. reflexivity.
+      }
+      intros ? ?.
+      rewrite interp_st_Ret. reflexivity.
+    }
+    setoid_rewrite map_bind.
+    repeat setoid_rewrite bind_Ret_l.
+    simpl.
+    unfold read_array_list_init.
+    reflexivity.
+    Defined.
+
+  Derive (swap_list12 : itree (exceptE Err) (list nat)) in
+    ( runST (S := S) (fun S => swap_first_and_last_list [1;2])
+        ≈
+      swap_list12
+    ) as tree_simplification5.
+  Proof.
+    unfold runST, swap_list12.
+    etransitivity.
+    { eapply eutt_fmap.
+      eapply (eutt_eq_bind_interp_st ltu ltac:(refine_prod)).
+      {
+        unfold newListArray. rewrite interp_st_trigger. cbn. reflexivity.
+      }
+      intros ? ?.
+      eapply (eutt_eq_bind_interp_st ltu ltac:(refine_prod)).
+      {
+        unfold swap_arr.
+        eapply (eutt_eq_bind_interp_st ltu ltac:(refine_prod)).
+        {
+          unfold readArray. rewrite interp_st_trigger. cbn. reflexivity.
+        }
+        intros ? ?.
+        eapply (eutt_eq_bind_interp_st ltu ltac:(refine_prod)).
+        {
+          unfold readArray. rewrite interp_st_trigger. cbn. reflexivity.
+        }
+        intros ? ?.
+        eapply (eutt_eq_bind_interp_st ltu ltac:(refine_prod)).
+        {
+          unfold writeArray. rewrite interp_st_trigger. cbn. reflexivity.
+        }
+        intros ? ?.
+        unfold writeArray. rewrite interp_st_trigger. cbn. reflexivity.
+      }
+      intros ? ?.
+      eapply (eutt_eq_bind_interp_st ltu ltac:(refine_prod)).
+      {
+        unfold getElems. rewrite interp_st_trigger. cbn. reflexivity.
+      }
+      intros ? ?.
+      rewrite interp_st_Ret. reflexivity.
+    }
+    setoid_rewrite map_bind.
+    repeat setoid_rewrite bind_Ret_l.
+    simpl.
+    reflexivity.
+    Defined.
+
+
+  Lemma sort_list2154 :
+    burn 10000 (runST (S := S) (fun S0 => sortList (S := S0) [2;1;5;4]))
+    = Ret [1;2;4;5].
+  Proof using Type. lazy. reflexivity. Qed.
+
+  Lemma sort_list__long :
+    burn 10000 (runST (S := S) (fun S0 => sortList (S := S0) [8;4;6;9;7;3;1;2;5]))
+    = Ret [1;2;3;4;5;6;7;8;9].
+  Proof using Type. lazy. reflexivity. Qed.
+
+
+End DeriveProofs.
