tests/monadic/stmonad/STMonadExamples.v
@@ -1,0 +1,253 @@
+From Crane Require Import Monads.STMonad.   
+
+From Stdlib Require Import
+  Arith.PeanoNat
+  Arith.Peano_dec
+  Init.Peano
+  List
+  Morphisms
+  RelationClasses
+  Relation_Definitions
+  Setoid
+  Strings.String
+  Classes.EquivDec
+  Basics
+.
+
+From Crane Require Import Monads.ITree.
+From ExtLib Require Import
+  CmpDec
+  Data.Bool
+  Data.List
+  Data.Map.FMapAList
+  Data.Monads.EitherMonad
+  Data.Pair
+  Data.String
+  Structures.Functor
+  Structures.Maps
+  Structures.Traversable
+  Structures.Reducible
+.
+
+
+From ITree Require Import
+  Events.Exception
+  Events.FailFacts
+  Events.MapDefault
+  Events.MapDefaultFacts
+  Events.State
+  Events.StateFacts
+  ITree
+  ITreeFacts
+.
+
+Import Monads.
+Import ListNotations.
+Import ProperNotations.
+Local Open Scope monad_scope.
+Local Open Scope string_scope.
+
+Section NatExampleTrees.
+
+  Context {T S : Type}.
+  Context {ltu : T -> T -> Prop}.
+  Context `{Ix_Correct T ltu}.
+  Context {HST: STRefClass T}.
+
+  Let V : T -> Type := fun _ => nat. (* Nats only for this example. *)
+  Let E0 := (STEvent T S V) +' exceptE Err.
+
+
+  Definition new_and_read_both_nat : itree E0 (nat * nat) :=
+      r1 <- newSTRef zero 5 ;;
+      r2 <- newSTRef (suc zero) 6 ;; (* TODO: autogenerate successive indices? *)
+      x1 <- readSTRef r1 ;;
+      x2 <- readSTRef r2 ;;
+      Ret (x1, x2).
+
+  Definition tree_simp_nat : itree E0 nat :=
+    v <- newSTRef zero 5;;
+    readSTRef v.
+
+  (* NOTE: this failing definition is intentional.
+    The intent is to test that we don't allow reference indices to escape. *)
+  Fail Definition tree_escape_nat : itree E0 nat :=
+    v <- newSTRef 5;;
+    writeSTRef v (match v with mkSTRef _ _ idx => idx end);;
+    readSTRef v.
+
+  Definition tree_simp_another_nat : itree E0 nat :=
+    v <- newSTRef zero 5;;
+    writeSTRef v 6;;
+    val <- readSTRef v;;
+    Ret val.
+
+
+   Definition swap' (v w : STRef S nat) : itree E0 unit :=
+    a <- @readSTRef E0 T S  _ V  _ (STRefToIx _ _ v) v;;
+    b <- @readSTRef E0 T S _ V _ (STRefToIx _ _ w) w;;
+    writeSTRef v b;;
+    writeSTRef w a.
+
+  (* "swap" function from "Lazy Functional State Threads", by John Launchbury and Simon L Peyton Jones. *)
+  (* TODO: would be good for indices here to be inferrable. *)
+  Fail Definition swap (v w : STRef S nat) : itree E0 unit :=
+    a <- readSTRef v;;
+    b <- readSTRef w;;
+    writeSTRef v b;;
+    writeSTRef w a.
+
+
+  Definition array_simp_fixed_init : itree E0 nat :=
+    arr <- newArray zero zero (suc (suc (suc (suc (suc zero))))) 5;;
+    elem <- @readArray E0 T _ _ _ _ _ arr (suc (zero));;
+    Ret elem. 
+  
+  Definition array_simp_list : itree E0 (nat * nat * list nat) :=
+    arr <- newListArray zero zero (suc (suc (suc zero))) [5;4;3;2];;
+    elem <- @readArray _ _ _ _ _ _ zero arr zero;;
+    lst <- @getElems _ _ _ _ _ _ zero arr;;
+    Ret (elem, length lst, lst). 
+
+
+
+  (* source: https://wiki.haskell.org/Monad/ST *)
+  (* TODO: should not have to manually place indices as arguments. *)
+  Definition fibST (n : nat) : itree E0 nat :=
+    let fix fibST' (n : nat) (x y : STRef S nat) (idx_x idx_y : T) : itree E0 nat :=
+      match n with
+      | 0 => @readSTRef _ _ _ _ _ _ idx_x x
+      | Datatypes.S n =>
+          x' <- @readSTRef _ _ _  _ _ _ idx_x x;;
+          y' <- @readSTRef _ _ _ _ _ _ idx_y y;;
+          @writeSTRef _ _ _ _ _ _ idx_x x y';;
+          @writeSTRef _ _ _ _ _ _ idx_y y (x' + y');;
+          fibST' n x y idx_x idx_y
+      end in
+    if (Nat.leb n 2)
+    then Ret n
+    else
+      x <- newSTRef zero 0;;
+      y <- newSTRef (suc zero) 1;;
+      fibST' n x y zero (suc zero).
+
+  Definition fibFun (n : nat) : nat :=
+    let fix fib' (n : nat) :=
+      match n with
+      | 0 => 0
+      | 1 => 1
+      | Datatypes.S (Datatypes.S m as m0) => fib' m0 + fib' m
+      end in
+    fib' n.
+
+  Section QSort. 
+
+
+    Definition swap_arr
+       {E' : Type -> Type}
+      `{STEvent T S V -< E'}
+      `{exceptE Err -< E'}
+      (arr : STArray T S nat) (arr_idx : T) (left : T) (right : T) : itree E' unit :=
+      leftVal <- readArray arr left;;
+      rightVal <- readArray arr right;;
+      @writeArray _ T S _ _ _ arr_idx arr left rightVal;;
+      @writeArray _ T S _ _ _ arr_idx arr right leftVal.
+
+  
+    Definition swap_first_and_last_list
+       {E' : Type -> Type}
+      `{STEvent T S V -< E'}
+      `{exceptE Err -< E'}
+      (xs : list nat) : itree E' (list nat) :=
+      let lastIndex := fromNat (length xs - 1) in 
+      arr <- newListArray zero zero lastIndex xs;;
+      swap_arr arr zero zero lastIndex;;
+      newXs <- getElems arr;;
+      Ret newXs.
+
+    Definition forEachWith {A B}
+       {E' : Type -> Type}
+      `{STEvent T S V -< E'}
+      `{exceptE Err -< E'}
+      (xs : list A) (v : B) (f : B -> A -> itree E' B)
+      : itree E' B :=
+      foldM (flip f) (Ret v) (rev xs). (* reversing so foldM goes left to right. *)
+
+
+    Definition partition 
+       {E' : Type -> Type}
+      `{STEvent T S V -< E'}
+      `{exceptE Err -< E'}
+      (arr : STArray T S nat) (arr_idx : T) (left : T) (right : T) (pivotIndex : T) : itree E' T :=
+      pivotValue <- @readArray _ _ _ _ _ _ arr_idx arr pivotIndex;;
+      swap_arr arr arr_idx pivotIndex right;;
+      storeIndex <- forEachWith (range left (sub right (suc zero))) left (fun storeIndex i =>
+          val <- @readArray _ _ _ _ _ _ arr_idx arr i;;
+          if (Nat.leb val pivotValue)
+              then swap_arr arr arr_idx i storeIndex;;
+                  Ret (suc storeIndex)
+              else Ret storeIndex );;
+      swap_arr arr arr_idx storeIndex right;;
+      Ret storeIndex.
+
+
+    (* NOTE: could define totally with equations, using a measure of the distance between pivots. *)
+    Definition qsort_body 
+      (args : (STArray T S nat * T * T * T))
+      : itree ((callE (STArray T S nat * T * T * T) unit) +' E0) unit :=
+      let '(arr,arr_idx,l,r) := args in
+      if (Nat.ltb (toNat l) (toNat r)) then
+        let leftn := toNat l in
+        let rightn := toNat r in 
+        let pivotIndexn := leftn + ((rightn - leftn) / 2) in
+        newPivot <- partition arr arr_idx l r (fromNat pivotIndexn);;
+        call (arr, arr_idx, l, (fromNat ((toNat newPivot) - 1)));;
+        call (arr, arr_idx, (fromNat ((toNat newPivot) + 1)), r)
+      else Ret tt.
+
+
+    Definition qsort (arr : STArray T S nat) (arr_idx : T) (left : T) (right : T) : itree E0 unit :=
+      rec qsort_body (arr, arr_idx, left, right).
+
+
+      (* arr <- newListArray zero zero (suc (suc (suc zero))) [5;4;3;2];; *)
+    Definition sortList (xs : list nat) : itree E0 (list nat) :=
+      let lastIndex := fromNat (length xs - 1) in 
+      arr <- newListArray zero zero lastIndex xs;;
+      qsort arr zero zero lastIndex;;
+      newXs <- getElems arr;;
+      Ret newXs.
+  
+
+  End QSort.
+
+  
+End NatExampleTrees.
+
+
+
+
+Section BoolExampleTrees.
+
+  Context {E : Type -> Type}.
+  Context {T S : Type}.
+  Context {ltu : T -> T -> Prop}.
+  Context `{Ix_Correct T ltu}.
+  Context {HST: STRefClass T}.
+
+  Let V : T -> Type := fun _ => bool. (* bools only for this example. *)
+  Let E0 := (STEvent T S V) +' exceptE Err.
+
+
+  Definition new_and_read_both_bool : itree E0 (bool * bool) :=
+      r1 <- newSTRef zero false ;;
+      r2 <- newSTRef (suc zero) true ;; 
+      x1 <- readSTRef r1 ;;
+      x2 <- readSTRef r2 ;;
+      Ret (x1, x2).
+
+  Definition tree_simp_bool : itree E0 bool :=
+    v <- newSTRef zero true;;
+    readSTRef v.
+
+End BoolExampleTrees.
